Knot proof with invariant style

examples/knot/KnotHeader.v
@@ -8,6 +8,7 @@ Require Import PCM.
 Require Import HoareDef.
 Require Import TODOYJ.
 Require Import Logic YPM.
+Require Import HTactics.
 
 Set Implicit Arguments.
 
@@ -16,39 +17,229 @@ Set Implicit Arguments.
 
 
 
-Definition invRA: URA.t := Auth.t (Excl.t unit).
-Definition inv_black : (@URA.car invRA) := Auth.black (M:=(Excl.t unit)) (Some tt).
-Definition inv_white : (@URA.car invRA) := Auth.white (M:=(Excl.t unit)) (Some tt).
 
 Section AUX.
+  Definition invRA: URA.t := Auth.t (Excl.t (Any.t * Any.t)).
+  Definition inv_black (mp_src mp_tgt: Any.t): (@URA.car invRA)
+    := Auth.black (M:=(Excl.t _)) (Some (mp_src, mp_tgt)).
+  Definition inv_white (mp_src mp_tgt: Any.t): (@URA.car invRA)
+    := Auth.white (M:=(Excl.t _)) (Some (mp_src, mp_tgt)).
+
   Context `{Σ: GRA.t}.
   Context `{@GRA.inG invRA Σ}.
 
-  Definition inv_open: iProp := OwnM inv_black.
-  Definition inv_closed: iProp := OwnM inv_white.
+  Definition inv_opener: iProp :=
+    (∃ mp_src mp_tgt, OwnM (inv_white mp_src mp_tgt))%I.
+  Definition inv_closed: iProp :=
+    (∃ mp_src mp_tgt, OwnM (inv_black mp_src mp_tgt))%I.
+  Definition inv_closer (mp_src mp_tgt: Any.t): iProp :=
+    OwnM (inv_black mp_src mp_tgt)%I.
+  Definition inv_open (mp_src mp_tgt: Any.t): iProp :=
+    OwnM (inv_white mp_src mp_tgt)%I.
 
-  Lemma inv_closed_unique
+
+
+  Lemma inv_opening mp_src mp_tgt
     :
-      inv_closed -∗ inv_closed -∗ False
-  .
+      inv_opener -∗ inv_closed -∗ #=> (inv_closer mp_src mp_tgt ** inv_open mp_src mp_tgt).
   Proof.
+    unfold inv_opener, inv_closed, inv_open, inv_closer, inv_white, inv_black.
     iIntros "H0 H1".
-    unfold inv_closed, inv_white in *.
-    iCombine "H0 H1" as "H". iOwnWf "H". iPureIntro.
-    repeat ur in H0. ss.
+    iDestruct "H0" as (mp_src0 mp_tgt0) "H0".
+    iDestruct "H1" as (mp_src1 mp_tgt1) "H1".
+    iCombine "H1 H0" as "H".
+    iPoseProof (OwnM_Upd with "H") as "H".
+    { instantiate (1:=Auth.black (Some (mp_src, mp_tgt): Excl.t _) ⋅ Auth.white (Some (mp_src, mp_tgt): Excl.t _)).
+      eapply Auth.auth_update. ii. des. split.
+      { ur. ss. }
+      { ur. ur in FRAME. des_ifs. }
+    }
+    { iMod "H". iModIntro. iDestruct "H" as "[H0 H1]". iFrame. }
   Qed.
 
-  Lemma inv_open_unique
+  Lemma inv_closing mp_src0 mp_tgt0 mp_src1 mp_tgt1
     :
-      inv_open -∗ inv_open -∗ False
+      inv_closer mp_src0 mp_tgt0 -∗ inv_open mp_src1 mp_tgt1 -∗ #=> (inv_opener ** inv_closed).
+  Proof.
+    unfold inv_opener, inv_closed, inv_open, inv_closer, inv_white, inv_black.
+    iIntros "H0 H1".
+    iCombine "H0 H1" as "H".
+    iPoseProof (OwnM_Upd with "H") as "H".
+    { instantiate (1:=Auth.black (Some (mp_src0, mp_tgt0): Excl.t _) ⋅ Auth.white (Some (mp_src0, mp_tgt0): Excl.t _)).
+      eapply Auth.auth_update. ii. des. split.
+      { ur. ss. }
+      { ur. ur in FRAME. des_ifs. }
+    }
+    { iMod "H". iDestruct "H" as "[H0 H1]".
+      iModIntro. iSplitL "H1".
+      { iExists _, _. ss. }
+      { iExists _, _. ss. }
+    }
+  Qed.
+
+  Lemma inv_open_unique mp_src mp_tgt
+    :
+      inv_opener -∗ inv_open mp_src mp_tgt -∗ False
   .
   Proof.
-    iIntros "H0 H1".
-    unfold inv_open, inv_black in *.
-    iCombine "H0 H1" as "H". iOwnWf "H". iPureIntro.
-    repeat ur in H0. ss.
+    unfold inv_opener, inv_closed, inv_open, inv_closer, inv_white, inv_black.
+    iIntros "H0 H1". iDestruct "H0" as (mp_src0 mp_tgt0) "H0".
+    iCombine "H0 H1" as "H". iOwnWf "H" as WF. exfalso.
+    repeat ur in WF. ss.
   Qed.
+
+  Lemma inv_close_unique mp_src mp_tgt
+    :
+      inv_closer mp_src mp_tgt -∗ inv_closed -∗ False
+  .
+  Proof.
+    unfold inv_opener, inv_closed, inv_open, inv_closer, inv_white, inv_black.
+    iIntros "H0 H1". iDestruct "H1" as (mp_src0 mp_tgt0) "H1".
+    iCombine "H0 H1" as "H". iOwnWf "H" as WF. exfalso.
+    repeat ur in WF. ss.
+  Qed.
+
+  Lemma inv_merge mp_src0 mp_tgt0 mp_src1 mp_tgt1
+    :
+      inv_closer mp_src0 mp_tgt0 -∗ inv_open mp_src1 mp_tgt1 -∗ ⌜mp_src1 = mp_src0 /\ mp_tgt1 = mp_tgt0⌝
+  .
+  Proof.
+    unfold inv_opener, inv_closed, inv_open, inv_closer, inv_white, inv_black.
+    iIntros "H0 H1".
+    iCombine "H0 H1" as "H". iOwnWf "H" as WF. iPureIntro.
+    eapply Auth.auth_included in WF. des.
+    eapply Excl.extends in WF; ss.
+    - des; clarify.
+    - ur; ss.
+  Qed.
+
+  Definition inv_wf
+             A
+             (R_src: A -> Any.t -> Any.t -> iProp)
+             (R_tgt: A -> Any.t -> Any.t -> iProp)
+    : (((Σ * Any.t)) * ((Σ * Any.t)) -> Prop) :=
+    @mk_wf
+      _
+      (A + Any.t * Any.t)
+      (fun a' mp_src mp_tgt =>
+         match a' with
+         | inl a => inv_closed ** R_src a mp_src mp_tgt
+         | inr (mp_src1, mp_tgt1) => inv_open mp_src1 mp_tgt1 ** ⌜mp_src1 = mp_src /\ mp_tgt1 = mp_tgt⌝
+         end)%I
+      (fun a' mp_src mp_tgt =>
+         match a' with
+         | inl a => R_tgt a mp_src mp_tgt
+         | inr (mp_src, mp_tgt) => top1
+         end)
+  .
+
+  Definition mk_inv_simple {X: Type} (PQ: X -> ((Any.t -> ord -> iProp) * (Any.t -> iProp))): fspec :=
+    mk_simple
+      (fun (x: X) =>
+         ((fun varg o =>
+             inv_opener
+               **
+               (fst (PQ x) varg o)),
+          (fun vret =>
+             inv_opener
+               **
+               (snd (PQ x) vret)))
+      ).
 End AUX.
+
+Ltac iarg :=
+  let PRE := constr:("PRE") in
+  let INV := constr:("INV") in
+  let OPENER := constr:("☃OPENER") in
+  let CLOSED := constr:("☃CLOSED") in
+  let ARG := constr:("ARG") in
+  eapply (@harg_clo _ PRE INV);
+  [eassumption
+  |
+  ];
+  let a := fresh "a" in
+  intros a; i;
+  mDesSep PRE as PRE ARG;
+  let EQ := fresh "EQ" in
+  mPure ARG as EQ;
+  try (destruct EQ);
+  mDesSep PRE as OPENER PRE;
+  destruct a as [?|[?mp_src ?mp_tgt]]; simpl;
+  [mDesSep INV as CLOSED INV
+  |mAssertPure False; ss; iDestruct "INV" as "[INV _]"; iApply (inv_open_unique with "☃OPENER INV")].
+
+Ltac open_inv :=
+  mAssert _ with "☃OPENER ☃CLOSED" as "☃TMP";
+  [ iApply (inv_opening with "☃OPENER ☃CLOSED"); fail
+   |mUpd "☃TMP"; mDesSep "☃TMP" as "☃CLOSER" "☃OPEN"].
+
+Ltac close_inv :=
+  mAssert _ with "☃CLOSER ☃OPEN" as "☃TMP";
+  [ iApply (inv_closing with "☃CLOSER ☃OPEN"); fail
+   |mUpd "☃TMP"; mDesSep "☃TMP" as "☃OPENER" "☃CLOSED"].
+
+Tactic Notation "icall_open" uconstr(o) uconstr(x) "with" constr(Hns) :=
+  let POST := get_fresh_name_tac "POST" in
+  let INV := constr:("☃OPEN") in
+  let Hns := select_ihyps Hns in
+  let Hns := constr:("☃OPEN"::Hns) in
+  eapply (@hcall_clo _ Hns POST INV o _ x _ (inr (_, _)));
+  unshelve_goal;
+  [eassumption
+  |
+  |start_ipm_proof; iFrame "☃OPEN"; iSplitR; [ss|]
+  |eauto with ord_step
+  |
+  |on_current ltac:(fun H => try clear H);
+   intros ? ? ? ? ? ? [|[?mp_src ?mp_tgt]]; i; simpl;
+   on_current ltac:(fun H => simpl in H);
+   [mDesSep "☃OPEN" as "☃CLOSED" "☃TMP";
+    mAssertPure False; ss; iApply (inv_close_unique with "☃CLOSER ☃CLOSED")
+   |mDesSep "☃OPEN" as "☃OPEN" "☃TMP"; mPure "☃TMP" as [[] []]
+   ]
+  ].
+
+Tactic Notation "icall_weaken" uconstr(ftsp) uconstr(o) uconstr(x) uconstr(a) "with" constr(Hns) :=
+  let POST := get_fresh_name_tac "POST" in
+  let INV := get_fresh_name_tac "INV" in
+  let CLOSED := constr:("☃CLOSED") in
+  let OPENER := constr:("☃OPENER") in
+  let Hns := select_ihyps Hns in
+  let Hns := constr:("☃CLOSED"::"☃OPENER"::Hns) in
+  eapply (@hcall_clo_weaken _ Hns POST INV _ _ ftsp o x _ (inl a));
+  unshelve_goal;
+  [|
+   eassumption
+   |
+   |start_ipm_proof
+    ; iFrame "☃CLOSED ☃OPENER"
+   (* ; iSplitR; [ss|] *)
+   |eauto with ord_step
+   |
+   |on_current ltac:(fun H => try clear H);
+    intros ? ? ? ? ? ? [|[?mp_src ?mp_tgt]]; i; simpl;
+    on_current ltac:(fun H => simpl in H);
+    [mDesSep INV as "☃CLOSED" INV;
+     mDesSep POST as POST "☃TMP";
+     let EQ := fresh in
+     mPure "☃TMP" as EQ; inversion EQ;
+     mDesSep POST as "☃OPENER" POST
+    |mDesSep INV as "☃CLOSED" INV;
+     mDesSep POST as POST "☃TMP";
+     mDesSep POST as "☃OPENER" POST;
+     mAssertPure False; [iApply (inv_open_unique with "☃OPENER ☃CLOSED")|ss
+    ]]
+  ].
+
+Tactic Notation "iret" uconstr(a) :=
+  eapply (@hret_clo _ _ (inl a)); unshelve_goal;
+  [eauto with ord_step
+  |eassumption
+  |
+  |start_ipm_proof; iFrame "☃CLOSED ☃OPENER"
+  |
+  ].
+
 
 
 Definition knotRA: URA.t := Auth.t (Excl.t (option (nat -> nat))).
@@ -59,7 +250,6 @@ Definition knot_init: (@URA.car knotRA) := knot_frag None.
 
 Section REC.
   Context `{Σ: GRA.t}.
-  Context `{@GRA.inG invRA Σ}.
 
   Definition mrec_spec (f: nat -> nat) (INV: iProp): ftspec (list val) val :=
     mk_simple (X:=nat)
